@prefix rdf: <http://www.w3.org/1999/02/22-rdf-syntax-ns#> .
@prefix rdfs: <http://www.w3.org/2000/01/rdf-schema#> .

# Affordance types

#How this affordances map to protocol actions is application dependent. By way
#of a concrete example, however, consider HTTP:
#GET Navigation, Embed
#OPTIONS/HEAD Metadata
#PUT Update
#DELETE Remove
#POST Create
#PATCH Mutate

<Affordance> a rdfs:Class ;
  rdfs:comment "Base class for all affordances" .

<Null> a rdfs:Class ;
  rdfs:subClassOf <Affordance> ;
  rdfs:comment "The provided affordance is null. i.e. not dereferenceable, no actions provided".

<Safe> a rdfs:Class ;
  rdfs:subClassOf <Affordance> ;
  rdfs:comment "A safe affordance - it is asserted that no change will be triggered by activating the affordance" .

<Navigation> a rdfs:Class ;
  rdfs:subClassOf <Safe> ;
  rdfs:comment """A link to another resource. The assumption
    is that otherwise undescribed URLs have a navigation affordance""" .

<Embed> a rdfs:Class ;
  rdfs:subClassOf <Safe>
  rdfs:comment "A resource that should be properly displayed in-line rather than provided as a hyperlink" .

<Metadata> a rdfs:Class ;
  rdfs:subClassOf <Safe> ;
  rdfs:comment "There is extra metadata available about this resource" .

<Idempotent> a rdfs:Class ;
  rdfs:subClassOf <Affordance>
  rdfs:comment "An affordance that will cause a change, but that can be repeated without further hazard" .

<Update> a rdfs:Class ;
  rdfs:subClassOf <Idempotent> ;
  rdfs:comment "Acting on this affordance will update the targeted resource. Repeated updates will have not further effect" .

<Remove> a rdfs:Class ;
  rdfs:subClassOf <Idempotent> ;
  rdfs:comment "Triggering this affordance is a request to delete the resource" .

<Unsafe> a rdfs:Class ;
  rdfs:subClassOf <Affordance>
  rdfs:comment "Affordances whose effects cannot be simply modeled and should be triggered with care" .

<Create> a rdfs:Class ;
  rdfs:subClassOf <Unsafe> ;
  rdfs:comment """Triggering this affordance implies a request to create a new
  resource""" .

<Mutate> a rdfs:Class ;
  rdfs:subClassOf <Unsafe> ;
  rdfs:comment """Triggering this affordance expresses a desire to make changes
  to a resource""" .

# Controls

<controlledBy> a rdf:Property ;
  rdfs:domain <Affordance>
  rdfs:range <Control>

<Control> a rdfs:Class .

<controlName> a rdf:Property
  rdfs:domain <Control> ;
  rdfs:range rdfs:Literal ;
  rdfs:comment "Valid values are limited per application. Examples include
  'Media-Type', 'Encoding' or 'EntityTag'"

<controlValue> a rdf:Property ;
  rdfs:domain <Control> ;
  rdfs:range rdfs:Literal .

# Authorization

<authorizedBy> a rdf:Property ;
  rdfs:domain <Affordance> ;
  rdfs:range rdfs:Resource ;
  rdfs:comment """Opaque descriptors of authorization tokens - resource can be
  dereferenced by users with that token. It's recommended that the tokens be
  defreferenceable, and that they be accessible iff the user is authorized to
  activate the affordance in question.""" .

# Target

<target> a rdf:Property ;
  rdfs:domain <Affordance> ;
  rdfs:range rdfs:Resource ;
  rdfs:range rdfs:Literal ;
  rdfs:comment "Could be a templated URL, or a URL resource. If not a template,
  but the Affordance has one or more uriVariable properties, the implication is
  that the target resource should be used as the basis of a URI template by
  appending (?name,other,...) to the URI." .

<uriVariable> a rdf:Property ;
  rdfs:domain <Affordance> ;
  rdfs:range <Parameter> ;
  rdfs:range rdf:List ;
  rdfs:comment """When the object is list, the members of the list should be
  Parameters, the the list order implies the order in which the parameters
  should be used""" .


<Parameter> a rdfs:Class .

<parameterName> a rdf:Property ;
  rdfs:domain Parameter ;
  rdfs:range Literal .

<parameterRange> a rdf:Property ;
  rdfs:domain Parameter ;
  rdfs:range Class .

# Payload

<payload> a rdf:Property ;
  rdfs:domain <Affordance> ;
  rdfs:range rdfs:Resource ;
  rdfs:comment """Points to a node in an isolated graph or to the name of a
  named graph that describes the possible payload of the affordance. Graph
  might need a different entailment - allowing e.g. a blank node to be the
  object of a property whose domain is Literal... i.e. only using RDF
  entailment, not RDFS""" .
