@base <http://judsonlester.info/affordance> .
@prefix rdf: <http://www.w3.org/1999/02/22-rdf-syntax-ns#> .
@prefix rdfs: <http://www.w3.org/2000/01/rdf-schema#> .

<#Affordance> a rdfs:Class ;
  rdfs:comment "Base class for all affordances" .

<#Null> a rdfs:Class ;
  rdfs:subClassOf <#Affordance> ;
  rdfs:comment "The provided affordance is null. i.e. not dereferenceable, no actions provided".

<#Safe> a rdfs:Class ;
  rdfs:subClassOf <#Affordance> ;
  rdfs:comment "A safe affordance - it is asserted that no change will be triggered by activating the affordance" .

<#Metadata> a rdfs:Class ;
  rdfs:subClassOf <#Safe> ;
  rdfs:comment "There is extra metadata available about this resource" .

<#Idempotent> a rdfs:Class ;
  rdfs:subClassOf <#Affordance> ;
  rdfs:comment "An affordance that will cause a change, but that can be repeated without further hazard" .

<#Unsafe> a rdfs:Class ;
  rdfs:subClassOf <#Affordance> ;
  rdfs:comment "Affordances whose effects cannot be simply modeled and should be triggered with care" .

<#Navigate> a rdfs:Class ;
  rdfs:subClassOf <#Safe> ;
  rdfs:comment "A link to another resource. The assumption is that otherwise undescribed URLs have a navigation affordance" .

<#Embed> a rdfs:Class ;
  rdfs:subClassOf <#Safe> ;
  rdfs:comment "A resource that should be properly displayed in-line rather than provided as a hyperlink" .

<#Update> a rdfs:Class ;
  rdfs:subClassOf <#Idempotent> ;
  rdfs:comment "Acting on this affordance will update the targeted resource. Repeated updates will have not further effect" .

<#Remove> a rdfs:Class ;
  rdfs:subClassOf <#Idempotent> ;
  rdfs:comment "Triggering this affordance is a request to delete the resource" .

<#Create> a rdfs:Class ;
  rdfs:subClassOf <#Unsafe> ;
  rdfs:comment """Triggering this affordance implies a request to create a new
  resource""" .

<#Mutate> a rdfs:Class ;
  rdfs:subClassOf <#Unsafe> ;
  rdfs:comment """Triggering this affordance expresses a desire to make changes
  to a resource""" .

#Consider: <#Append> - distinct from <#Create> in that the implication is
#specifically to create a child (or otherwise related) resource to the target, where <#Create> might
#specifically mean "create this resource" - review Fielding & 2616

# Controls

<#controlledBy> a rdf:Property ;
  rdfs:domain <#Affordance> ;
  rdfs:range <#Control> .

<#Control> a rdfs:Class .

<#controlName> a rdf:Property ;
  rdfs:domain <#Control> ;
  rdfs:range rdfs:Literal ;
  rdfs:comment "Valid values are limited per application. Examples include 'Media-Type', 'Encoding' or 'EntityTag'" .

<#controlValue> a rdf:Property ;
  rdfs:domain <#Control> ;
  rdfs:range rdfs:Literal .

# Authorization

<#authorizedBy> a rdf:Property ;
  rdfs:domain <#Affordance> ;
  rdfs:range rdfs:Resource ;
  rdfs:comment """Opaque descriptors of authorization tokens - resource can be
  dereferenced by users with that token. It's recommended that the tokens be
  defreferenceable, and that they be accessible iff the user is authorized to
  activate the affordance in question.""" .

# Target

<#target> a rdf:Property ;
  rdfs:domain <#Affordance> ;
  rdfs:range rdfs:Resource ;
  rdfs:comment """Could be a templated URL, or a URL resource. If not a template,
  but the Affordance has one or more uriVariable properties, the implication is
  that the target resource should be used as the basis of a URI template by
  appending (?name,other,...) to the URI.""" .

# Payload

<#ResourceTemplate> a rdfs:Class .

<#pattern> a rdf:Property ;
  rdfs:domain <#ResourceTemplate> ;
  rdfs:range rdfs:Literal ;
  rdfs:comment """An IRITemplate (RFC 5xxx) that defines how the template is
    rendered - implicitly, all the parameters of the template are provided as a
    key, value set called param_list, so something like (?param_list*) should
    work like an HTML action=GET form""" .

<#var> a rdf:Property ;
  rdfs:domain <#ResourceTemplate> ;
  rdfs:range <#LiteralTemplate> , rdf:List ;
  rdfs:comment """When the object is list, the members of the list should be
    Parameters, the the list order implies the order in which the parameters
    should be used""" .

<#LiteralTemplate> a rdfs:Class .

<#name> a rdf:Property ;
  rdfs:domain <#LiteralTemplate> ;
  rdfs:range rdfs:Literal .

<#label> a rdf:Property ;
  rdfs:domain <#LiteralTemplate> ;
  rdfs:range rdfs:Literal .

<#range> a rdf:Property ;
  rdfs:domain <#LiteralTemplate> ;
  rdfs:range rdfs:Class .

<#defaultValue> a rdf:Property ;
  rdfs:domain <#LiteralTemplate> ;
  rdfs:domain rdfs:Resource .

#Omittable vs required values?

<#subjectTemplate> a rdf:Property ;
  rdfs:domain rdf:Statement ;
  rdfs:range <#ResourceTemplate> ;
  rdfs:comment """Used to indicate that a resource template can be used as the
  subject in a statement""" .

<#predicateTemplate> a rdf:Property ;
  rdfs:domain rdf:Statement ;
  rdfs:range <#ResourceTemplate> ;
  rdfs:comment """Used to indicate that a resource template can be used as the
  property in a statement""" .

<#objectTemplate> a rdf:Property ;
  rdfs:domain rdf:Statement ;
  rdfs:range <#ResourceTemplate> , <#LiteralTemplate> ;
  rdfs:comment """Used to indicate that a resource or literal template can be
  used
  as the property in a statement""" .

<#payload> a rdf:Property ;
  rdfs:domain <#Affordance> ;
  rdfs:range rdfs:Resource .

<#statement> a rdf:Property ;
  rdfs:domain rdfs:Resource ;
  rdfs:range rdf:Statement .
