@base <http://judsonlester.info/rdf-vocab/path> .
@prefix rdf: <http://www.w3.org/1999/02/22-rdf-syntax-ns#> .
@prefix rdfs: <http://www.w3.org/2000/01/rdf-schema#> .

<#Step> a rdfs:Class ;
  rdfs:comment "Base class for path steps" .

<#RepeatingStep> a rdfs:Class ;
  rdfs:subClassOf <#Step> ;
  rdfs:comment "A step that repeats - the subject of a matching step become the subject of a new match" .

<#MultipleStep> a rdfs:Class ;
  rdfs:subClassOf <#Step> ;
  rdfs:comment "A step that may appear more than once on a subject" .

<#Root> a rdfs:Class ;
  rdfs:comment "The starting point of a path pattern" .

<#Target> a rdfs:Class ;
  rdfs:comment "A target for the pattern" .

<#Literal> a rdfs:Class ;
  rdfs:subClassOf <#Target> .

<#forward> a rdf:Property ;
  rdfs:domain <#Step> , <#Root> ;
  rdfs:range <#Step> ;
  rdfs:comment """Indicates that the subject of the matched statement matches the
                  subject, and the predicate of the matched statement matches the
                  predicate.""" .

<#reverse> a rdf:Property ;
  rdfs:domain <#Step> , <#Root> ;
  rdfs:range <#Step> ;
  rdfs:comment """Indicates that the subject of the matched statement matches the
                  predicate, and the predicate of the matched statement matches the
                  subject.""" .

<#predicate> a rdf:Property ;
  rdfs:domain <#Step> ;
  rdfs:range rdfs:Resource ;
  rdfs:comment "The property of a statement that matches this step" .

<#minRepeat> a rdf:Property ;
  rdfs:domain <#RepeatingStep> ;
  rdfs:range rdfs:Literal ; #specify integer?
  rdfs:comment """Limits the number of times a repeating step may repeat - otherwise
                  a repeating step is assumed allow 0 repetions.""" .

<#maxRepeat> a rdf:Property ;
  rdfs:domain <#RepeatingStep> ;
  rdfs:range rdfs:Literal ; #specify integer?
  rdfs:comment """Limits the number of times a repeating step may repeat - otherwise
                  a repeating step is assumed to have no limit to repetitions.""" .

<#minMulti> a rdf:Property ;
  rdfs:domain <#FanStep> ;
  rdfs:range rdfs:Literal ; #specify integer?
  rdfs:comment """Limits the number of times a repeating step may repeat - otherwise
                  a repeating step is assumed allow 0 repetions.""" .

<#maxMulti> a rdf:Property ;
  rdfs:domain <#FanStep> ;
  rdfs:range rdfs:Literal ; #specify integer?
  rdfs:comment """Limits the number of times a repeating step may repeat - otherwise
                  a repeating step is assumed to have no limit to repetitions.""" .

<#name> a rdf:Property ;
  rdfs:domain <#Target> ;
  rdfs:range rdfs:Literal .

<#label> a rdf:Property ;
  rdfs:domain <#Target> ;
  rdfs:range rdfs:Literal .

<#type> a rdf:Property ;
  rdfs:domain <#Literal> ;
  rdfs:range rdfs:Class .

<#constraint> a rdf:Property ;
  rdfs:domain <#Literal> ;
  rdfs:range rdfs:Literal ;
  rdfs:comment "Description of constraints on values that can match this Literal." .

<#order> a rdf:Property ;
  rdfs:domain <#Literal> ;
  rdfs:range rdfs:Resource ;
  rdfs:comment """The subject resource describes the order in which to consider values of this
                  Literal.""" .

<#after> a rdf:Property ;
  rdfs:domain <#Literal> ;
  rdfs:range rdfs:Resource ;
  rdfs:comment """Constrains the matching of this literal to values that come after the subject
                  value in some order.""" .

<#before> a rdf:Property ;
  rdfs:domain <#Literal> ;
  rdfs:range rdfs:Resource ;
  rdfs:comment """Constrains the matching of this literal to values that come before the subject
                  value in some order.""" .

<#defaultValue> a rdf:Property ;
  rdfs:domain <#Literal> ;
  rdfs:range rdfs:Resource .

<#numeric> a rdf:Value ;
  rdfs:comment """An order value which simply means that values for the Literal in
                  question should be considered in normal numeric order. Application to
                  non-numeric values is undefined.""" .

<#alpha> a rdf:Value ;
  rdfs:comment """Literals considered in alphabetic order are sorted in natural alphabetic
                  order in the natural language of the literal. e.g. In English, A > a > B > b""" .
